code_pairing_imp

theories/ExamplePairingHeap.v
@@ -10,8 +10,63 @@ License: MIT.
 *)
 
 Set Implicit Arguments.
-From TLC Require Import LibCore LibMultiset.
+From TLC Require Import LibCore.
+From Sep Require Import Example.
+From Sep Require Import ExampleList.
 
+
+(* ******************************************************* *)
+(** ** Mutable lists extension *)
+
+Module MList.
+
+Parameter MListOf : forall A `{EA:Enc A} TA (R:TA->A->hprop) (L:list TA) (p:loc), hprop.
+(*
+  \exists v, p ~~> v \*
+  match L with
+  | nil => \[v = Nil]
+  | x::L' => \exists X p', \[v = Cons x p'] \* (x ~> RA X) \* (p' ~> MList L')
+  end.
+*)
+
+Section Ops.
+
+Context A {EA:Enc A} TA (R:TA->A->hprop).
+Implicit Types L : list TA.
+Implicit Types p : loc.
+Implicit Types x : A.
+Implicit Types X : TA.
+
+Parameter is_empty : val.
+
+Parameter Triple_is_empty : forall L p,
+  TRIPLE (is_empty p)
+    PRE (p ~> MListOf R L)
+    POST (fun b => \[b = isTrue (L = nil)] \* p ~> MListOf R L).
+
+Parameter push : val.
+
+Parameter Triple_push : forall L p x X,
+  TRIPLE (push p ``x)
+    PRE (p ~> MListOf R L \* x ~> R X)
+    POST (fun (_:unit) => p ~> MListOf R (X::L)).
+
+Parameter pop : val.
+
+Parameter Triple_pop : forall L p,
+  L <> nil ->
+  TRIPLE (pop p)
+    PRE (p ~> MListOf R L)
+    POST (fun x => \exists X L', \[L = X::L'] \* x ~> R X \* p ~> MListOf R L').
+
+End Ops.
+
+End MList.
+
+
+(* ####################################################### *)
+
+From TLC Require Import LibMultiset.
 
 Tactic Notation "multiset_eq" := (* TODO: move to TLC *)
   check_noevar_goal; permut_simpl.
@@ -26,9 +81,7 @@ Notation "'elems'" := (multiset elem).
 
 
 (* ####################################################### *)
-(** * Purely functional pairing heaps *)
-
-Module PurePairing.
+(** * Data types and invariants *)
 
 
 (* ******************************************************* *)
@@ -40,45 +93,6 @@ Inductive heap : Type :=
 
 Instance Inhab_heap : Inhab heap.
 Proof using. applys Inhab_of_val Empty. Qed.
-
-
-(* ******************************************************* *)
-(** ** Operations *)
-
-Definition empty : heap :=
-  Empty.
-
-Definition is_empty (h:heap) : bool :=
-  match h with
-  | Empty => true
-  | _ => false
-  end.
-
-Definition merge (h1 h2:heap) : heap :=
-  match h1, h2 with
-   | _, Empty => h1
-   | Empty, _ => h2
-   | Node x hs1, Node y hs2 =>
-       If x < y
-          then Node x (h2::hs1)
-          else Node y (h1::hs2)
-   end.
-
-Definition insert (h:heap) (x:elem) : heap :=
-  merge (Node x nil) h.
-
-Fixpoint merge_pairs (hs:list heap) : heap :=
-  match hs with
-  | nil => Empty
-  | h::nil => h
-  | h1::h2::hs' => merge (merge h1 h2) (merge_pairs hs')
-  end.
-
-Definition pop_min (h:heap) : elem * heap :=
-  match h with
-  | Node x hs => (x, merge_pairs hs)
-  | _ => arbitrary
-  end.
 
 
 (* ******************************************************* *)
@@ -162,6 +176,60 @@ Proof using.
   { autos*. }
 Qed.
 
+Lemma pop_min_lemma : forall x Es,
+  Forall (foreach (is_ge x)) Es ->
+  min_of (\{x} \u list_union Es) x.
+Proof.
+  introv M. split. 
+  { auto. }
+  { intros y Hy. multiset_in Hy.
+    { auto. }  { applys* Forall_foreach_is_ge_inv Es. } }
+Qed.
+
+
+(* ####################################################### *)
+(** * Purely functional pairing heaps *)
+
+Module PurePairing.
+
+(* ******************************************************* *)
+(** ** Coq code *)
+
+Definition empty : heap :=
+  Empty.
+
+Definition is_empty (h:heap) : bool :=
+  match h with
+  | Empty => true
+  | _ => false
+  end.
+
+Definition merge (h1 h2:heap) : heap :=
+  match h1, h2 with
+   | _, Empty => h1
+   | Empty, _ => h2
+   | Node x hs1, Node y hs2 =>
+       If x < y
+          then Node x (h2::hs1)
+          else Node y (h1::hs2)
+   end.
+
+Definition insert (h:heap) (x:elem) : heap :=
+  merge (Node x nil) h.
+
+Fixpoint merge_pairs (hs:list heap) : heap :=
+  match hs with
+  | nil => Empty
+  | h::nil => h
+  | h1::h2::hs' => merge (merge h1 h2) (merge_pairs hs')
+  end.
+
+Definition pop_min (h:heap) : elem * heap :=
+  match h with
+  | Node x hs => (x, merge_pairs hs)
+  | _ => arbitrary
+  end.
+
 
 (* ******************************************************* *)
 (** ** Verification *)
@@ -216,11 +284,11 @@ Proof using.
       unfold list_union. rew_listx.
       applys_eq merge_spec 1.
       { applys* merge_spec. }
-      { applys* IH. Search tclosure. hnf; rew_list*. }
+      { applys* IH. hnf; rew_list*. }
       { autos*. } } }
 Qed.
 
-Lemma delete_min_spec : forall h E h' x,
+Lemma pop_min_spec : forall h E h' x,
   E <> \{} ->
   inv h E ->
   (x,h') = pop_min h ->
@@ -230,14 +298,109 @@ Proof using.
   introv N I M. unfolds pop_min.
   destruct h as [|y hs]; inverts I; tryfalse.
   { invert M ;=> <- Eh'. forwards* Is: merge_pairs_spec hs. split.
-    { unfold min_of. split.
-      { auto. }
-      { intros y Hy. multiset_in Hy. { auto. } 
-        { applys* Forall_foreach_is_ge_inv Es. } } }
-    { eauto. } }
+    { applys* pop_min_lemma. } { eauto. } }
 Qed.
 
 End PurePairing.
+
+
+(* ####################################################### *)
+(** * Imperative ephemeral pairing heaps *)
+
+
+
+Module ImperativePairing.
+
+
+(* ******************************************************* *)
+(** ** OCaml+null code *)
+
+(**
+[[
+
+  type heap = ref node
+
+  type node = {
+    value : elem;
+    sub : heap mlist; }
+
+  let create() =
+    ref null
+
+	let is_empty p =
+		(!p == null)
+
+  let merge p1 p2 =
+		if is_empty p1 then p1 else
+		if is_empty p2 then p2 else
+		if (!p1.value < !p2.value) then (
+			push !p1.sub p2;
+			p1
+		) else (
+			push !p2.sub p1;
+			p2
+		)
+
+	let merge_pairs hs =
+    if is_empty hs then null else
+    let p1 = pop hs in
+    if is_empty hs then p1 else
+    let p2 = pop hs in
+		merge (merge p1 p2) (merge_pairs hs)
+
+	let pop_min p =
+    let x = !p.value in
+    p := merge_pairs (!p.sub);
+		x
+
+]]
+*)
+
+
+(* ******************************************************* *)
+(** ** Deeply embedded code *)
+
+Notation "''hs'" := ("hs":var) : var_scope.
+
+Definition value : field := 0%nat.
+Definition sub : field := 1%nat.
+
+Definition create : val :=
+  VFun 'u := 
+    val_ref null.
+
+Definition is_empty : val :=
+  VFun 'p := 
+    'p '= null.
+
+Definition merge : val :=
+  VFun 'p1 'p2 := 
+		If_ is_empty 'p1 Then 'p1 Else
+		If_ is_empty 'p2 Then 'p2 Else
+		If_ ('!'p1'.value '< '!'p2'.value) Then (
+			MList.push ('!'p1'.sub) 'p2 ';
+			'p1
+		) Else (
+			MList.push ('!'p2'.sub) 'p1 ';
+			'p2
+		).
+
+Definition merge_pairs : val :=
+  VFix 'f 'hs := 
+		If_ is_empty 'hs Then null Else
+    Let 'p1 := MList.pop 'hs in
+    If_ is_empty 'hs Then 'p1 Else
+    Let 'p2 := MList.pop 'hs in
+		merge (merge 'p1 'p2) ('f 'hs).
+
+Definition pop_min : val :=
+  VFun 'p :=
+    Let 'x := '!'p'.value in
+    'p ':= merge_pairs ('!'p'.sub) ';
+		'x.
+
+
+
 
 
 (* ####################################################### *)
@@ -258,201 +421,7 @@ Qed.
 *)
 
 
-(**
-
-
-
 (*
-
-Set Implicit Arguments.
-Require Import FuncTactics LibCore.
-Require Import OrderedSig_ml HeapSig_ml OrderedSig_proof HeapSig_proof.
-Require Import PairingHeap_ml.
-
-Module PairingHeapSpec (O:MLOrdered) (OS:OrderedSigSpec with Module O:=O)
-  <: HeapSigSpec with Definition H.MLElement.t := O.t.
-
-(** instantiations *)
-
-Module Import H <: MLHeap := MLPairingHeap O.
-Module Import OS := OS.
-Existing Instance le_inst.
-Existing Instance le_order.
-
-(** invariant *)
-
-Definition is_ge (X Y:T) := X <= Y.
-
-Definition list_union (Hs:list (multiset T)) := 
-  fold_right union \{} Hs.
-
-Inductive inv : heap -> multiset T -> Prop :=
-  | inv_empty : 
-      inv Empty \{} 
-  | inv_node : forall x X hs Hs E,
-      rep x X ->
-      Forall2 inv hs Hs ->
-      Forall (fun H => H <> \{}) Hs ->
-      Forall (foreach (is_ge X)) Hs ->
-      E = \{X} \u list_union Hs ->   
-      inv (Node x hs) E.
-
-(** model *)
-
-Fixpoint size (t:heap) : nat :=
-  match t with
-  | Empty => 1%nat
-  | Node x hs => (1 + (1 + List.fold_right (fun t x => (x + size t)%nat) 0%nat hs)%nat)%nat 
-  end.
-
-Instance heap_rep : Rep heap (multiset T).
-Proof.
-  apply (Build_Rep inv). intros x. gen_eq n: (size x). gen x.
-  induction n using peano_induction; introv N HX HY; 
-  subst n; inverts HX; inverts HY; subst. prove_rep.
-  fequals. prove_rep. fequals. clear X X0 H0 H2 H3 H6 H8 H9. gen Hs Hs0.
-  induction hs; introv K1 K2; inverts K1; inverts K2. prove_rep. fequals.
-  applys* H. simpl; math. applys~ IHhs. intros. applys* H. simpls. math. 
-Defined.
-
-(** automation *)
-
-Hint Extern 1 (_ < _) => simpl; math.
-Hint Extern 1 (_ = _ :> multiset _) => permut_simpl : multiset.
-Hint Unfold removed_min.
-
-Definition U := multiset T.
-
-Ltac myauto cont :=
-  match goal with 
-  | |- _ = _ :> LibSet.set ?T => try solve [ change (multiset T) with U; cont tt ]
-  | |- _ => cont tt
-  end.
-
-Ltac auto_tilde ::= myauto ltac:(fun _ => eauto).
-Ltac auto_star ::= try solve [ intuition (eauto with multiset) ].
-
-Hint Constructors inv Forall Forall2.
-
-(** useful facts *)
-
-Lemma foreach_ge_trans : forall (X Y : OS.T) (E : multiset OS.T),
-  foreach (is_ge X) E -> Y <= X -> foreach (is_ge Y) E.
-Proof. intros. apply~ foreach_weaken. intros_all. apply* le_trans. Qed.
-
-Hint Resolve foreach_ge_trans.
-
-Lemma min_of_prove : forall (X : OS.T) (Hs : list (multiset OS.T)),
-  Forall (foreach (is_ge X)) Hs ->
-  min_of ('{X} \u list_union Hs) X.
-Proof.
-  introv H. split~. introv M. destruct (in_union_inv M) as [N|N].
-  rewrite (in_single N). apply le_refl.
-  clear M. unfolds list_union. induction Hs; simpls.
-    false. eapply in_empty. eauto.
-    inversions H. destruct (in_union_inv N) as [P|P].
-      apply~ H3.
-      apply~ IHHs.
-Qed.
-
-Hint Resolve min_of_prove.
-
-(** verification *)
-
-Lemma empty_spec : rep empty \{}.
-Proof. apply empty_cf. xret~. Qed.
-
-Hint Extern 1 (RegisterSpec empty) => Provide empty_spec.
-
-Lemma is_empty_spec : RepTotal is_empty (E;heap) >> 
-  bool_of (E = \{}).
-Proof.
-  xcf. intros e E RepE. inverts RepE; xgo. 
-  auto. multiset_inv.
-Qed. 
-
-Hint Extern 1 (RegisterSpec is_empty) => Provide is_empty_spec.
-
-Lemma merge_spec : RepTotal merge (E1;heap) (E2;heap) >>
-  E1 \u E2 ;- heap.
-Proof.
-  xcf. introv Rep1 Rep2. xmatch.
-  xgo. inverts Rep2. equates* 1.
-  xgo. inverts Rep1. equates* 1.
-  xcleanpat. inverts keep Rep1. inverts keep Rep2. xgo~.
-    constructors.
-      eauto.
-      eauto. 
-      constructors~. multiset_inv.
-      clear H6 H7 Rep2. constructors. eauto. rew_foreach. splits~.
-       applys (@foreach_weaken _ (is_ge X0)).
-         unfold list_union. induction Hs0; simpl. auto. inverts~ H8.
-         intros_all. applys~ le_trans.
-    unfold list_union. simple*.
-    lets: (nle_to_sle P_x0). constructors.
-      eauto.
-      eauto. 
-      constructors~. multiset_inv.
-      clear H2 H3 Rep1. constructors. eauto. rew_foreach. splits~.
-       applys (@foreach_weaken _ (is_ge X)).
-         unfold list_union. induction Hs; simpl. auto. inverts~ H4.
-         intros_all. applys~ le_trans.
-    unfold list_union. simpl. permut_simpl.
-Qed.
-
-Hint Extern 1 (RegisterSpec merge) => Provide merge_spec.
-
-Lemma insert_spec : RepTotal insert (X;O.t) (E;heap) >>
-  \{X} \u E ;- heap.
-Proof.
-  xcf. introv RepX RepE. xapp~ (>>> \{X} E).
-  applys~ (>>> inv_node X (@nil (multiset T))).
-  unfolds list_union. simple*.
-Qed.
-
-Hint Extern 1 (RegisterSpec insert) => Provide insert_spec.
-
-Lemma merge_pairs_spec : Spec merge_pairs hs |R>>
-  forall Hs, 
-  Forall2 inv hs Hs ->
-  Forall (fun H => H <> \{}) Hs -> 
-  R (list_union Hs ;- heap).
-Proof.
-  xinduction (@List.length heap). xcf. introv IH RepH NE. xmatch.
-  xgo. inverts~ RepH.
-  xgo. inverts RepH. inverts H2. unfolds list_union. simpls. equates* 1.
-  xcleanpat. inverts RepH. inverts H2. inverts NE. inverts H2.
-   xgo~. ximpl. equates* 1.
-Qed.
-
-Hint Extern 1 (RegisterSpec merge_pairs) => Provide merge_pairs_spec.
-
-Lemma find_min_spec : RepSpec find_min (E;heap) |R>>
-  E <> \{} -> R (min_of E ;; O.t).
-Proof.
-  xcf. intros e E RepE HasE. inverts RepE; xgo*.
-Qed.
-
-Hint Extern 1 (RegisterSpec find_min) => Provide find_min_spec.
-
-Lemma delete_min_spec : RepSpec delete_min (E;heap) |R>>
-  E <> \{} -> R (removed_min E ;; heap).
-Proof. 
-  xcf. intros e E RepE HasE. inverts RepE; xgo~. ximpl. xrep~.
-Qed.
-
-Hint Extern 1 (RegisterSpec delete_min) => Provide delete_min_spec.
-
-End PairingHeapSpec.
-
-
-
-
-
-*)
-
-(*
-
 
 https://sites.google.com/site/progyumming/cpp/pairing-heap
 
@@ -462,87 +431,5 @@ https://www.sanfoundry.com/cpp-program-implement-pairing-heap/
 
 https://www.techiedelight.com/deletion-from-bst/
 
-
-module PairingHeap (Element : Ordered) : Heap =
-  (* (Heap with module Element = Element)*)
-struct
-  module Element = Element
-
-
-  type heap = Empty | Node of Element.t * heap list
-
-  let empty = Empty
-
-  let is_empty = function
-     | Empty -> true
-     | _ -> false
-
-  let merge h1 h2 = 
-     match h1, h2 with
-     | _, Empty -> h1
-     | Empty, _ -> h2
-     | Node (x, hs1), Node (y, hs2) ->
-         if Element.leq x y 
-            then Node (x, h2 :: hs1)
-            else Node (y, h1 :: hs2)
-
-  let insert x h = 
-     merge (Node (x, [])) h
-
-  let rec merge_pairs = function
-     | [] -> Empty
-     | [h] -> h
-     | h1::h2::hs -> merge (merge h1 h2) (merge_pairs hs)
-
-  let find_min = function 
-     | Empty -> raise EmptyStructure 
-     | Node (x, _) -> x
-
-  let delete_min = function 
-     | Empty -> raise EmptyStructure 
-     | Node (x, hs) -> merge_pairs hs
-
-end
-
-
-
-type pairing_heap = ref node
-
-  create() =
-    ref null
-
-	let is_empty p =
-		return (!p == null)
-
-	let pop_front p =
-		if (empty p) fail
-    int x = !p.value;
-    root = merge_pairs(!p->sub);
-		return x
-
-type node = { 
-		int value;
-		node* parent;
-		mlist<node*> sub;
-};
-
-let merge(node * a, node * b)  : node* =
-		if (a == null) return b;
-		if (b == null) return a;
-		if (!a.value < !b.value) {
-			!a.sub.push_front(b);
-			return a;
-		} else {
-			!b.sub.push_front(a);
-			return b;
-		}
-	}
-	node * merge_pairs(list<node*> s) {
-    if s.is_empty() return null else
-    let a = s.pop_front()
-    if s.is_empty() return a else
-    let b = s.pop_front()
-		return merge(merge(a, b), merge_pairs(s));
-	}
 
 *)
